You are solving math problems by carefully identifying the cause-and-effect relationships and constraints in the problem. For each question, reason causally about what conditions must be true, what steps logically follow from them, and how they lead to the final answer. Avoid jumping to conclusions; instead, analyze what causes what. Follow the instruction format to use dollar sign to quote your final answer. Don't output anything after giving final answer.


Problem:
Find the domain of the expression $\\frac{\\sqrt{x-2}}{\\sqrt{5-x}}$.
Solution:
To determine the domain, we need to ensure the expression is defined. 
Causally, the square root $\\sqrt{x - 2}$ is defined only if $x - 2 \ge 0$ because taking the root of a negative number is undefined in the real numbers. So, this constraint causes the condition $x \ge 2$.
Similarly, the square root $\\sqrt{5 - x}$ in the denominator must be positive, not just non-negative, to avoid division by zero. So $5 - x > 0$, which causes the condition $x < 5$.
Combining both, the domain is all $x$ such that $2 \le x < 5$.
Final Answer: The final answer is $[2,5)$. I hope it is correct.


Problem:
If $\\det \\mathbf{A} = 2$ and $\\det \\mathbf{B} = 12,$ then find $\\det (\\mathbf{A} \\mathbf{B}).$
Solution:
There is a causal rule in linear algebra: the determinant of the product of two matrices equals the product of their determinants. This means that the values of $\\det \\mathbf{A}$ and $\\det \\mathbf{B}$ cause the value of $\\det(\\mathbf{A}\\mathbf{B})$ through multiplication.
So, we compute $(\\det \\mathbf{A})(\\det \\mathbf{B}) = (2)(12) = 24$.
Final Answer: The final answer is $24$. I hope it is correct.


Problem:
Terrell usually lifts two 20-pound weights 12 times. If he uses two 15-pound weights instead, how many times must Terrell lift them in order to lift the same total weight?
Solution:
First, we identify what causes the total lifted weight: the number of repetitions and the weight of each lift.
Initially, the total lifted is $2 \\cdot 20 \\cdot 12 = 480$ pounds. 
Now, let the new number of reps be $n$. The causal relationship is: $2 \\cdot 15 \\cdot n = 30n$, which must equal 480 to maintain the same total.
Solving $30n = 480$ gives $n = 16$.
Final Answer: The final answer is $16$. I hope it is correct.


Problem:
If the system of equations
\begin{align*}
6x - 4y &= a,\\
6y - 9x &= b
\end{align*}
has a solution $(x, y)$ where $x$ and $y$ are both nonzero, find $\\frac{a}{b},$ assuming $b$ is nonzero.
Solution:
To relate $a$ and $b$, we consider how the equations interact. 
Multiply the first equation by $-\\frac{3}{2}$ to align its terms with the second:
$-\\frac{3}{2}(6x - 4y) = -9x + 6y = -\\frac{3}{2}a$.
The left-hand side is now identical to the second equation, which equals $b$.
So this causal equivalence gives $-\\frac{3}{2}a = b$, and rearranging gives $\\frac{a}{b} = -\\frac{2}{3}$.
Final Answer: The final answer is $-\\frac{2}{3}$. I hope it is correct.


Problem:
What is the largest digit $N$ for which $2345N$ is divisible by 6?
Solution:
To determine when $2345N$ is divisible by 6, we need to analyze the divisibility conditions causally.
There is a causal rule that a number is divisible by 6 if and only if it's divisible by both 2 and 3, because $6 = 2 \times 3$ and 2 and 3 are coprime.
For divisibility by 2, the last digit must be even. This constraint causes $N$ to be one of $\{0, 2, 4, 6, 8\}$.
For divisibility by 3, the sum of all digits must be divisible by 3. The sum is $2 + 3 + 4 + 5 + N = 14 + N$. Since $14 \equiv 2 \\pmod{3}$, we need $N \equiv 1 \\pmod{3}$ for the total sum to be divisible by 3. This constraint causes $N$ to be one of $\{1, 4, 7\}$.
The intersection of these two constraints gives us only $N = 4$, since it's the only digit that satisfies both conditions.
Therefore, the largest (and only) digit $N$ that satisfies both conditions is $4$.
Final Answer: The final answer is $4$. I hope it is correct.


Problem:
What is the intersection of the lines given by $2y=-x+3$ and $-y=5x+1$? Enter the answer as an ordered pair.
Solution:
To find the intersection, we need to determine the point where both equations are simultaneously satisfied.
From the second equation $-y = 5x + 1$, we can solve for $y$: $y = -5x - 1$. This establishes a causal relationship between $x$ and $y$.
Substituting this expression for $y$ into the first equation causes us to have one equation in one variable: $2(-5x - 1) = -x + 3$.
Expanding: $-10x - 2 = -x + 3$.
Collecting terms: $-10x + x = 3 + 2$, which gives $-9x = 5$.
This constraint causes $x = -\\frac{5}{9}$.
Substituting back into $y = -5x - 1$: $y = -5\left(-\\frac{5}{9}\right) - 1 = \\frac{25}{9} - 1 = \\frac{25}{9} - \\frac{9}{9} = \\frac{16}{9}$.
Therefore, the intersection point is $\left(-\\frac{5}{9}, \\frac{16}{9}\right)$.
Final Answer: The final answer is $\left(-\\frac{5}{9}, \\frac{16}{9}\right)$. I hope it is correct.


Problem:
Find the value of $x$ that satisfies $\\frac{\\sqrt{3x+5}}{\\sqrt{6x+5}}=\\frac{\\sqrt{5}}{3}$. Express your answer as a common fraction.
Solution:
To solve this equation, we need to eliminate the square roots while preserving equality.
First, we need the expressions under the square roots to be non-negative. This causal evidence requires $3x + 5 \geq 0$ and $6x + 5 \geq 0$, which give us $x \geq -\\frac{5}{3}$ and $x \geq -\\frac{5}{6}$ respectively. The more restrictive constraint is $x \geq -\\frac{5}{3}$.
Additionally, since we have $\\sqrt{6x+5}$ in the denominator, we need $6x + 5 > 0$, causing $x > -\\frac{5}{6}$.
To eliminate the square roots, we square both sides: $\left(\\frac{\\sqrt{3x+5}}{\\sqrt{6x+5}}\right)^2 = \left(\\frac{\\sqrt{5}}{3}\right)^2$.
This simplifies to: $\\frac{3x+5}{6x+5} = \\frac{5}{9}$.
Cross-multiplying: $9(3x+5) = 5(6x+5)$, which expands to $27x + 45 = 30x + 25$.
Rearranging: $45 - 25 = 30x - 27x$, causing $20 = 3x$.
Therefore, $x = \\frac{20}{3}$.
We can verify this satisfies our constraint $x > -\\frac{5}{6}$ since $\\frac{20}{3} > 0 > -\\frac{5}{6}$.
Final Answer: The final answer is $\\frac{20}{3}$. I hope it is correct.


Problem:
The fifth and eighth terms of a geometric sequence of real numbers are $7!$ and $8!$ respectively. What is the first term?
Solution:
In a geometric sequence, each term is caused by multiplying the previous term by a constant ratio $r$. The general term is $a_n = ar^{n-1}$, where $a$ is the first term.
Given information causes us to have:
- $a_5 = ar^4 = 7! = 5040$
- $a_8 = ar^7 = 8! = 40320$
To find the common ratio, we use the fact that $a_8 = a_5 \\cdot r^3$ (since we multiply by $r$ three more times to get from the 5th to the 8th term).
This causal relationship gives us: $\\frac{a_8}{a_5} = r^3 = \\frac{8!}{7!} = 8$.
Taking the cube root: $r = 2$.
Now, substituting $r = 2$ into the equation $ar^4 = 7!$:
$a \\cdot 2^4 = 5040$
$a \\cdot 16 = 5040$
This constraint causes $a = \\frac{5040}{16} = 315$.
Final Answer: The final answer is $315$. I hope it is correct.